- add record rules to the monoiu system

proof/uni_monoiu/algo_worklist/transfer.v
@@ -17,10 +17,10 @@ Open Scope dbind.
 
 Fixpoint ss_to_denv (θ : subst_set) : denv := 
   match θ with 
-  | nil => nil
-  | (X , dbind_tvar_empty) :: θ' => (X ~ dbind_tvar_empty) ++ ss_to_denv θ'
-  | (X , dbind_stvar_empty) :: θ' => (X ~ dbind_stvar_empty) ++ ss_to_denv θ'
-  | (X , dbind_typ T) :: θ' => ss_to_denv θ'
+    | nil => nil
+    | (X , dbind_tvar_empty) :: θ' => (X ~ dbind_tvar_empty) ++ ss_to_denv θ'
+    | (X , dbind_stvar_empty) :: θ' => (X ~ dbind_stvar_empty) ++ ss_to_denv θ'
+    | (X , dbind_typ T) :: θ' => ss_to_denv θ'
   end.
 
 Notation " ⌈ θ ⌉ᵈ " :=
@@ -71,6 +71,9 @@ Inductive trans_typ : subst_set -> typ -> typ -> Prop :=
   | trans_typ_unit : forall θ,
       wf_ss θ ->
       trans_typ θ typ_unit typ_unit
+  | trans_typ_label : forall θ l,
+      wf_ss θ ->
+      trans_typ θ (typ_label l) (typ_label l)
   | trans_typ__bot : forall θ,
       wf_ss θ ->
       trans_typ θ typ_bot typ_bot
@@ -94,8 +97,7 @@ Inductive trans_typ : subst_set -> typ -> typ -> Prop :=
   | trans_typ__union : forall θ A1ᵃ A2ᵃ A1ᵈ A2ᵈ,
       trans_typ θ A1ᵃ A1ᵈ ->
       trans_typ θ A2ᵃ A2ᵈ ->
-      trans_typ θ (typ_union A1ᵃ A2ᵃ) (typ_union A1ᵈ A2ᵈ)
-  . 
+      trans_typ θ (typ_union A1ᵃ A2ᵃ) (typ_union A1ᵈ A2ᵈ).
 
 Inductive trans_exp : subst_set -> exp -> exp -> Prop :=
   | trans_exp__unit : forall θ,
@@ -104,6 +106,16 @@ Inductive trans_exp : subst_set -> exp -> exp -> Prop :=
   | trans_exp__var : forall θ x,
       wf_ss θ ->
       trans_exp θ (exp_var_f x) (exp_var_f x)
+  | trans_exp__rcd_nil : forall θ,
+      wf_ss θ ->
+      trans_exp θ exp_rcd_nil exp_rcd_nil 
+  | trans_exp__rcd_cons : forall θ l1 e1ᵃ e1ᵈ e2ᵃ e2ᵈ,
+      trans_exp θ e1ᵃ e1ᵈ ->
+      trans_exp θ e2ᵃ e2ᵈ ->
+      trans_exp θ (exp_rcd_cons l1 e1ᵃ e2ᵃ) (exp_rcd_cons l1 e1ᵈ e2ᵈ)
+  | trans_exp__rcd_proj : forall θ l eᵃ eᵈ,
+      trans_exp θ eᵃ eᵈ ->
+      trans_exp θ (exp_rcd_proj eᵃ l) (exp_rcd_proj eᵈ l)
   | trans_exp__abs : forall L θ eᵃ eᵈ,
       (forall x, x ∉ L -> 
         trans_exp θ (open_exp_wrt_exp eᵃ (exp_var_f x))
@@ -131,38 +143,50 @@ Inductive trans_exp : subst_set -> exp -> exp -> Prop :=
 
 Inductive trans_conts : subst_set -> conts -> conts -> Prop :=
   | trans_conts__infabs : forall θ cdᵃ cdᵈ,
-    trans_contd θ cdᵃ cdᵈ ->
-    trans_conts θ (conts_infabs cdᵃ) (conts_infabs cdᵈ)
-  | trans_cont__inftapp : forall θ Aᵃ Aᵈ cᵃ cᵈ,
-    trans_typ θ Aᵃ Aᵈ ->
-    trans_conts θ cᵃ cᵈ ->
-    trans_conts θ (conts_inftapp Aᵃ cᵃ) (conts_inftapp Aᵈ cᵈ)
-  | trans_cont__inftappunion : forall θ A1ᵃ A1ᵈ A2ᵃ A2ᵈ cᵃ cᵈ,
-    trans_typ θ A1ᵃ A1ᵈ ->
-    trans_typ θ A2ᵃ A2ᵈ ->
-    trans_conts θ cᵃ cᵈ ->
-    trans_conts θ (conts_inftappunion A1ᵃ A2ᵃ cᵃ) (conts_inftappunion A1ᵈ A2ᵈ cᵈ)
-  | trans_cont__unioninftapp : forall θ Aᵃ Aᵈ cᵃ cᵈ,
-    trans_typ θ Aᵃ Aᵈ ->
-    trans_conts θ cᵃ cᵈ ->
-    trans_conts θ (conts_unioninftapp Aᵃ cᵃ) (conts_unioninftapp Aᵈ cᵈ)
+      trans_contd θ cdᵃ cdᵈ ->
+      trans_conts θ (conts_infabs cdᵃ) (conts_infabs cdᵈ)
+  | trans_conts__inftapp : forall θ Aᵃ Aᵈ csᵃ csᵈ,
+      trans_typ θ Aᵃ Aᵈ ->
+      trans_conts θ csᵃ csᵈ ->
+      trans_conts θ (conts_inftapp Aᵃ csᵃ) (conts_inftapp Aᵈ csᵈ)
+  | trans_conts__inftappunion : forall θ A1ᵃ A1ᵈ A2ᵃ A2ᵈ csᵃ csᵈ,
+      trans_typ θ A1ᵃ A1ᵈ ->
+      trans_typ θ A2ᵃ A2ᵈ ->
+      trans_conts θ csᵃ csᵈ ->
+      trans_conts θ (conts_inftappunion A1ᵃ A2ᵃ csᵃ) (conts_inftappunion A1ᵈ A2ᵈ csᵈ)
+  | trans_conts__unioninftapp : forall θ Aᵃ Aᵈ csᵃ csᵈ,
+      trans_typ θ Aᵃ Aᵈ ->
+      trans_conts θ csᵃ csᵈ ->
+      trans_conts θ (conts_unioninftapp Aᵃ csᵃ) (conts_unioninftapp Aᵈ csᵈ)
+  | trans_conts__infrcdconsintersection : forall θ l eᵃ eᵈ csᵃ csᵈ,
+      trans_exp θ eᵃ eᵈ ->
+      trans_conts θ csᵃ csᵈ ->
+      trans_conts θ (conts_infrcdconsintersection l eᵃ csᵃ) (conts_infrcdconsintersection l eᵈ csᵈ)
+  | trans_conts__intersectioninfrcdcons : forall θ Aᵃ Aᵈ csᵃ csᵈ,
+      trans_typ θ Aᵃ Aᵈ ->
+      trans_conts θ csᵃ csᵈ ->
+      trans_conts θ (conts_intersectioninfrcdcons Aᵃ csᵃ) (conts_intersectioninfrcdcons Aᵈ csᵈ)
   | trans_cont__sub : forall θ Aᵃ Aᵈ,
-    trans_typ θ Aᵃ Aᵈ ->
-    trans_conts θ (conts_sub Aᵃ) (conts_sub Aᵈ)
+      trans_typ θ Aᵃ Aᵈ ->
+      trans_conts θ (conts_sub Aᵃ) (conts_sub Aᵈ)
 with trans_contd : subst_set -> contd -> contd -> Prop :=
   | trans_contd__infapp : forall θ eᵃ eᵈ csᵃ csᵈ,
-    trans_exp θ eᵃ eᵈ ->
-    trans_conts θ csᵃ csᵈ ->
-    trans_contd θ (contd_infapp eᵃ csᵃ) (contd_infapp eᵈ csᵈ)
+      trans_exp θ eᵃ eᵈ ->
+      trans_conts θ csᵃ csᵈ ->
+      trans_contd θ (contd_infapp eᵃ csᵃ) (contd_infapp eᵈ csᵈ)
+  | trans_contd__infproj : forall θ Aᵃ Aᵈ csᵃ csᵈ,
+      trans_typ θ Aᵃ Aᵈ ->
+      trans_conts θ csᵃ csᵈ ->
+      trans_contd θ (contd_infproj Aᵃ csᵃ) (contd_infproj Aᵈ csᵈ)
   | trans_contd__infabs_union : forall θ Aᵃ Aᵈ cdᵃ cdᵈ,
-    trans_typ θ Aᵃ Aᵈ ->
-    trans_contd θ cdᵃ cdᵈ ->
-    trans_contd θ (contd_infabsunion Aᵃ cdᵃ) (contd_infabsunion Aᵈ cdᵈ)
+      trans_typ θ Aᵃ Aᵈ ->
+      trans_contd θ cdᵃ cdᵈ ->
+      trans_contd θ (contd_infabsunion Aᵃ cdᵃ) (contd_infabsunion Aᵈ cdᵈ)
   | trans_contd__unioninfabs : forall θ Aᵃ Aᵈ Bᵃ Bᵈ cdᵃ cdᵈ,
-    trans_typ θ Aᵃ Aᵈ ->
-    trans_typ θ Bᵃ Bᵈ ->
-    trans_contd θ cdᵃ cdᵈ ->
-    trans_contd θ (contd_unioninfabs Aᵃ Bᵃ cdᵃ) (contd_unioninfabs Aᵈ Bᵈ cdᵈ).
+      trans_typ θ Aᵃ Aᵈ ->
+      trans_typ θ Bᵃ Bᵈ ->
+      trans_contd θ cdᵃ cdᵈ ->
+      trans_contd θ (contd_unioninfabs Aᵃ Bᵃ cdᵃ) (contd_unioninfabs Aᵈ Bᵈ cdᵈ).
 
 Inductive trans_work : subst_set -> work -> work -> Prop :=
   | trans_work__inf : forall θ eᵃ eᵈ csᵃ csᵈ,
@@ -189,6 +213,12 @@ Inductive trans_work : subst_set -> work -> work -> Prop :=
       trans_exp θ eᵃ eᵈ ->
       trans_conts θ csᵃ csᵈ ->
       trans_work θ (work_infapp Aᵃ Bᵃ eᵃ csᵃ) (work_infapp Aᵈ Bᵈ eᵈ csᵈ)
+  | trans_work__infproj : forall θ Aᵃ Aᵈ Bᵃ Bᵈ Cᵃ Cᵈ csᵃ csᵈ,
+      trans_typ θ Aᵃ Aᵈ ->
+      trans_typ θ Bᵃ Bᵈ ->
+      trans_typ θ Cᵃ Cᵈ ->
+      trans_conts θ csᵃ csᵈ ->
+      trans_work θ (work_infproj Aᵃ Bᵃ Cᵃ csᵃ) (work_infproj Aᵈ Bᵈ Cᵈ csᵈ)
   | trans_work__inftapp : forall θ A1ᵃ A1ᵈ A2ᵃ A2ᵈ csᵃ csᵈ,
       trans_typ θ A1ᵃ A1ᵈ ->
       trans_typ θ A2ᵃ A2ᵈ ->
@@ -216,6 +246,16 @@ Inductive trans_work : subst_set -> work -> work -> Prop :=
       trans_typ θ B2ᵃ B2ᵈ ->
       trans_contd θ cdᵃ cdᵈ ->
       trans_work θ (work_unioninfabs A1ᵃ B1ᵃ A2ᵃ B2ᵃ cdᵃ) (work_unioninfabs A1ᵈ B1ᵈ A2ᵈ B2ᵈ cdᵈ)
+  | trans_work__infrcdconsintersection : forall θ l1 A1ᵃ A1ᵈ e2ᵃ e2ᵈ csᵃ csᵈ,
+      trans_typ θ A1ᵃ A1ᵈ ->
+      trans_exp θ e2ᵃ e2ᵈ ->
+      trans_conts θ csᵃ csᵈ ->
+      trans_work θ (work_infrcdconsintersection l1 A1ᵃ e2ᵃ csᵃ) (work_infrcdconsintersection l1 A1ᵈ e2ᵈ csᵈ)
+  | trans_work__intersectioninfrcdcons : forall θ A1ᵃ A1ᵈ A2ᵃ A2ᵈ csᵃ csᵈ,
+      trans_typ θ A1ᵃ A1ᵈ ->
+      trans_typ θ A2ᵃ A2ᵈ ->
+      trans_conts θ csᵃ csᵈ ->
+      trans_work θ (work_intersectioninfrcdcons A1ᵃ A2ᵃ csᵃ) (work_intersectioninfrcdcons A1ᵈ A2ᵈ csᵈ)
   | trans_work__applys : forall θ Aᵃ Aᵈ csᵃ csᵈ,
       trans_typ θ Aᵃ Aᵈ ->
       trans_conts θ csᵃ csᵈ ->
@@ -224,9 +264,9 @@ Inductive trans_work : subst_set -> work -> work -> Prop :=
       trans_typ θ Aᵃ Aᵈ ->
       trans_typ θ Bᵃ Bᵈ ->
       trans_contd θ cdᵃ cdᵈ ->
-      trans_work θ (work_applyd cdᵃ Aᵃ Bᵃ) (work_applyd cdᵈ Aᵈ Bᵈ)
-.
+      trans_work θ (work_applyd cdᵃ Aᵃ Bᵃ) (work_applyd cdᵈ Aᵈ Bᵈ).
 
+      
 Notation "θ ᵗ⊩ Aᵃ ⇝ Aᵈ" := (trans_typ θ Aᵃ Aᵈ)
   (at level 65, Aᵃ at next level, no associativity).
 
@@ -668,48 +708,7 @@ Qed.
 
 #[local] Hint Resolve trans_typ_wf_ss : core.
 #[local] Hint Resolve trans_typ_lc_atyp trans_typ_lc_dtyp : core.
-
-
-Lemma trans_typ_neq_all : forall θ Aᵃ Aᵈ,
-  θ ᵗ⊩ Aᵃ ⇝ Aᵈ -> 
-  neq_all Aᵃ -> 
-  neq_all Aᵈ.
-Proof.
-  intros. dependent destruction H0; dependent destruction H; eauto.
-  + apply wf_ss_binds_mono_typ in H0; auto.
-    eapply d_mono_typ_neq_all. eauto.
-Qed.
-
-Lemma trans_typ_neq_all_rev : forall θ Aᵃ Aᵈ,
-  θ ᵗ⊩ Aᵃ ⇝ Aᵈ -> 
-  neq_all Aᵈ -> 
-  neq_all Aᵃ.
-Proof.
-  intros. dependent destruction H0; dependent destruction H; eauto.
-Qed.
-
-Lemma trans_typ_neq_union_rev : forall θ Aᵃ Aᵈ,
-  θ ᵗ⊩ Aᵃ ⇝ Aᵈ -> 
-  neq_union Aᵈ ->
-  neq_union Aᵃ.
-Proof.
-  intros. dependent destruction H0; dependent destruction H; eauto.
-Qed.
-
-Lemma trans_typ_neq_intersection_rev : forall θ Aᵃ Aᵈ,
-  θ ᵗ⊩ Aᵃ ⇝ Aᵈ -> 
-  neq_intersection Aᵈ -> 
-  neq_intersection Aᵃ.
-Proof.
-  intros. dependent destruction H0; dependent destruction H; eauto.
-Qed.
-
-#[export] Hint Resolve 
-  trans_typ_neq_all trans_typ_neq_all_rev 
-  trans_typ_neq_union_rev trans_typ_neq_intersection_rev
-  : core.
   
-
 Lemma trans_typ_det : forall θ Aᵃ A₁ᵈ A₂ᵈ,
   uniq θ -> 
   θ ᵗ⊩ Aᵃ ⇝ A₁ᵈ -> 
@@ -733,7 +732,7 @@ Ltac unify_trans_typ :=
       eauto; subst
   end.
 
-  Lemma trans_exp_det : forall θ eᵃ e₁ᵈ e₂ᵈ,
+Lemma trans_exp_det : forall θ eᵃ e₁ᵈ e₂ᵈ,
   uniq θ -> 
   θ ᵉ⊩ eᵃ ⇝ e₁ᵈ -> 
   θ ᵉ⊩ eᵃ ⇝ e₂ᵈ -> 
@@ -741,6 +740,8 @@ Ltac unify_trans_typ :=
 Proof with eauto.
   intros * Huniq Htrans1 Htrans2. generalize dependent e₂ᵈ.
   induction Htrans1; (intros; dependent destruction Htrans2; auto).
+  - apply f_equal3...
+  - apply f_equal2... 
   - inst_cofinites_by (L `union` L0 `union` (fvar_in_exp eᵈ) `union` (fvar_in_exp eᵈ0) `union`  dom θ) using_name x.
     apply f_equal.
     eapply open_exp_wrt_exp_inj with (x1:=x); auto.  
@@ -777,10 +778,13 @@ Proof with eauto.
     + apply f_equal2... unify_trans_typ.
     + apply f_equal3; repeat unify_trans_typ. 
     + apply f_equal2... unify_trans_typ.
+    + apply f_equal3... unify_trans_exp.
+    + apply f_equal2... unify_trans_typ.
     + apply f_equal. unify_trans_typ.
   - intros. generalize dependent cd₂ᵈ.
     induction H0; (intros cd₂ᵈ Htrans2; dependent destruction Htrans2).
     + apply f_equal2... unify_trans_exp.
+    + apply f_equal2... unify_trans_typ.
     + apply f_equal2... unify_trans_typ.
     + apply f_equal3; repeat unify_trans_typ.
 Qed.
@@ -1084,7 +1088,7 @@ Proof with eauto.
 Qed.
 
 Lemma trans_typ_dtvar_dtyp_s_in_atyp : forall θ X Aᵃ Aᵈ b,
-  b = dbind_tvar_empty \/ b = dbind_stvar_empty ->
+  b = □ \/ b = ■ ->
   θ ᵗ⊩ Aᵃ ⇝ Aᵈ ->
   binds X b θ ->
   (forall Y T, Y ~ T ∈ᵈ θ -> Y `in` ftvar_in_typ Aᵃ -> X `in` ftvar_in_typ T -> False) ->
@@ -1356,6 +1360,8 @@ Proof with auto.
     eapply wf_ss_rename_tvar; eauto.
   - constructor.
     eapply wf_ss_rename_tvar; eauto.
+  - constructor...
+    eapply wf_ss_rename_tvar; eauto.
   - inst_cofinites_for trans_exp__abs.
     intros. inst_cofinites_with x.
     eapply H0 in H1; eauto.
@@ -1440,8 +1446,6 @@ Ltac solve_trans_exp_open_close' :=
   match goal with
   | H : ?θ ᵉ⊩ ?e1ᵃ ⇝ ?eᵈ |- ?θ' ᵉ⊩ ?e2ᵃ ⇝ ({(exp_var_f ?x1') ᵉ/ₑ ?x} ?eᵈ) => 
       eapply trans_exp_rename_var with (x:=x) (x':=x1') in H
-  (* | H : ?θ ᵉ⊩ ?e1ᵃ ⇝ ?eᵈ |- ?θ' ᵉ⊩ ?e2ᵃ ⇝ ({(exp_var_f ?x') ᵉ/ₑ ?x} ?eᵈ) => 
-      assert (θ ᵉ⊩ e1ᵃ ⇝ eᵈ) by admit *)
   end.
 
 Ltac solve_s_in' :=
@@ -1508,9 +1512,7 @@ Lemma trans_exp_total : forall θ Γ Ω eᵃ,
   nil ⊩ Γ ⇝ Ω ⫣ θ -> 
   exists eᵈ, trans_exp θ eᵃ eᵈ.
 Proof with eauto using trans_typ_total.
-  intros. generalize dependent Ω. 
-  generalize dependent θ. 
-  dependent induction H; intros...
+  intros. generalize dependent Ω. generalize dependent θ. dependent induction H; intros...
   - pick fresh x. 
     eapply trans_typ_total in H...
     destruct H as [Tᵈ].
@@ -1546,7 +1548,15 @@ Proof with eauto using trans_typ_total.
       intros. destruct_conj...
     } 
     apply Hex...
-Qed.
+  - assert (Hex: (exists e1ᵈ, θ ᵉ⊩ e1 ⇝ e1ᵈ) -> (exists e2ᵈ, θ ᵉ⊩ e2 ⇝ e2ᵈ) -> exists eᵈ, θ ᵉ⊩ exp_rcd_cons l e1 e2 ⇝ eᵈ). {
+      intros. destruct_conj...
+    } 
+    apply Hex...
+  - assert (Hex: (exists eᵈ, θ ᵉ⊩ e ⇝ eᵈ) -> exists eᵈ, θ ᵉ⊩ exp_rcd_proj e l ⇝ eᵈ). {
+      intros. destruct_conj...
+    } 
+    apply Hex...
+ Qed.
 
 Lemma trans_conts_total : forall θ Γ Ω csᵃ,
   ⌊ Γ ⌋ᵃ ᶜˢ⊢ᵃ csᵃ ->  
@@ -1580,6 +1590,14 @@ Proof with eauto using trans_typ_total, trans_exp_total.
         intros. destruct_conj...
       }
       apply Hex...
+    + assert (Hex: (exists eᵈ, θ ᵉ⊩ e ⇝ eᵈ) -> (exists csᵈ, θ ᶜˢ⊩ cs ⇝ csᵈ) -> exists csᵈ, θ ᶜˢ⊩ conts_infrcdconsintersection l e cs ⇝ csᵈ). {
+        intros. destruct_conj...
+      }
+      apply Hex...
+    + assert (Hex: (exists Aᵈ, θ ᵗ⊩ A ⇝ Aᵈ) -> (exists csᵈ, θ ᶜˢ⊩ cs ⇝ csᵈ) -> exists csᵈ, θ ᶜˢ⊩ conts_intersectioninfrcdcons A cs ⇝ csᵈ). {
+        intros. destruct_conj...
+      }
+      apply Hex...
     + assert (Hex: (exists Aᵈ, θ ᵗ⊩ A ⇝ Aᵈ) -> exists csᵈ, θ ᶜˢ⊩ conts_sub A ⇝ csᵈ). {
         intros. destruct_conj...
       }
@@ -1603,6 +1621,10 @@ Proof with eauto using trans_typ_total, trans_exp_total.
         intros. destruct_conj...
       }
       dependent destruction H.
+      apply Hex...
+    + assert (Hex:  (exists Aᵈ, θ ᵗ⊩ A ⇝ Aᵈ) -> (exists csᵈ, θ ᶜˢ⊩ cs ⇝ csᵈ) -> exists cdᵈ, θ ᶜᵈ⊩ contd_infproj A cs ⇝ cdᵈ). {
+        intros. destruct_conj...
+      }
       apply Hex...
 Qed.
 
@@ -1650,52 +1672,9 @@ Proof.
     destruct H as [T].  
     eapply binds_ss_etvar_binds_ss_to_aenv; eauto.
   - dependent destruction Htransa; eauto.
+  - econstructor.
   - dependent destruction Htransa; eauto.
   - dependent destruction Htransa; eauto.
-Qed.
-
-Lemma trans_wl_a_wneq_all_d_wneq_all : forall Γ Ω θ Aᵃ Aᵈ,
-  nil ⊩ Γ ⇝ Ω ⫣ θ ->
-  θ ᵗ⊩ Aᵃ ⇝ Aᵈ -> 
-  a_wneq_all (⌊ Γ ⌋ᵃ) Aᵃ -> 
-  d_wneq_all (⌊ Ω ⌋ᵈ) Aᵈ.
-Proof with eauto using a_wneq_all, d_wneq_all.
-  intros * Htranswl Htrans Hneq. generalize dependent Aᵈ.
-  dependent induction Hneq; intros; dependent destruction Htrans; eauto...
-  - econstructor...
-    eapply trans_wl_a_wl_binds_tvar_d_wl...
-  - eapply trans_wl_a_wl_binds_tvar_ss in Htranswl...
-    unify_binds.
-  - eapply trans_wl_a_wl_binds_tvar_ss in Htranswl...
-    unify_binds.
-  - eapply trans_wl_a_wl_binds_etvar_ss in Htranswl...
-    destruct Htranswl as [T]. 
-    unify_binds.
-  - eapply trans_wl_a_wl_binds_etvar_ss in Htranswl...
-    destruct Htranswl as [T]. 
-    unify_binds.
-  - apply wf_ss_binds_mono_typ in H1; auto.
-    eapply trans_wl_ss_mono_typ_d_wl_mono_typ in H1...
-    eapply d_mono_typ_d_wneq_all...
-Qed.
-
-Lemma trans_wl_d_wneq_all_a_wneq_all : forall Γ Ω θ Aᵃ Aᵈ,
-  nil ⊩ Γ ⇝ Ω ⫣ θ ->
-  θ ᵗ⊩ Aᵃ ⇝ Aᵈ -> 
-  d_wneq_all (⌊ Ω ⌋ᵈ) Aᵈ ->
-  a_wneq_all (⌊ Γ ⌋ᵃ) Aᵃ. 
-Proof with eauto using a_wneq_all, d_wneq_all.
-  intros * Htranswl Htrans Hneq. generalize dependent Aᵃ.
-  dependent induction Hneq; intros; dependent destruction Htrans; eauto;
-    try solve [eapply trans_wl_ss_binds_etvar_a_wl in H0; eauto using a_wneq_all, d_wneq_all].
-  - econstructor. 
-    eapply trans_wl_ss_binds_tvar_a_wl...
-  - eapply trans_wl_d_wl_binds_tvar_ss in H...
-    apply binds_ss_to_denv_binds_ss in H. unify_binds.
-  - eapply trans_wl_ss_binds_etvar_a_wl in H1...
-  - eapply trans_wl_ss_binds_etvar_a_wl in H2...
-  - eapply trans_wl_ss_binds_etvar_a_wl in H1...
-  - eapply trans_wl_ss_binds_etvar_a_wl in H1...
 Qed.
 
 Lemma trans_typ_binds_etvar : forall θ X T,
@@ -1792,6 +1771,50 @@ Proof.
   eapply trans_typ_tvar_stvar_in_etvar_binds_in_atyp'; eauto.
 Qed.
 
+Lemma trans_wl_a_wneq_all_d_wneq_all : forall Γ Ω θ Aᵃ Aᵈ,
+  nil ⊩ Γ ⇝ Ω ⫣ θ ->
+  θ ᵗ⊩ Aᵃ ⇝ Aᵈ -> 
+  a_wneq_all (⌊ Γ ⌋ᵃ) Aᵃ -> 
+  d_wneq_all (⌊ Ω ⌋ᵈ) Aᵈ.
+Proof with eauto using a_wneq_all, d_wneq_all.
+  intros * Htranswl Htrans Hneq. generalize dependent Aᵈ.
+  dependent induction Hneq; intros; dependent destruction Htrans; eauto...
+  - econstructor...
+    eapply trans_wl_a_wl_binds_tvar_d_wl...
+  - eapply trans_wl_a_wl_binds_tvar_ss in Htranswl...
+    unify_binds.
+  - eapply trans_wl_a_wl_binds_tvar_ss in Htranswl...
+    unify_binds.
+  - eapply trans_wl_a_wl_binds_etvar_ss in Htranswl...
+    destruct Htranswl as [T]. 
+    unify_binds.
+  - eapply trans_wl_a_wl_binds_etvar_ss in Htranswl...
+    destruct Htranswl as [T]. 
+    unify_binds.
+  - apply wf_ss_binds_mono_typ in H1; auto.
+    eapply trans_wl_ss_mono_typ_d_wl_mono_typ in H1...
+    eapply d_mono_typ_d_wneq_all...
+Qed.
+
+Lemma trans_wl_d_wneq_all_a_wneq_all : forall Γ Ω θ Aᵃ Aᵈ,
+  nil ⊩ Γ ⇝ Ω ⫣ θ ->
+  θ ᵗ⊩ Aᵃ ⇝ Aᵈ -> 
+  d_wneq_all (⌊ Ω ⌋ᵈ) Aᵈ ->
+  a_wneq_all (⌊ Γ ⌋ᵃ) Aᵃ. 
+Proof with eauto using a_wneq_all, d_wneq_all.
+  intros * Htranswl Htrans Hneq. generalize dependent Aᵃ.
+  dependent induction Hneq; intros; dependent destruction Htrans; eauto;
+    try solve [eapply trans_wl_ss_binds_etvar_a_wl in H0; eauto using a_wneq_all, d_wneq_all].
+  - econstructor. 
+    eapply trans_wl_ss_binds_tvar_a_wl...
+  - eapply trans_wl_d_wl_binds_tvar_ss in H...
+    apply binds_ss_to_denv_binds_ss in H. unify_binds.
+  - eapply trans_wl_ss_binds_etvar_a_wl in H1...
+  - eapply trans_wl_ss_binds_etvar_a_wl in H2...
+  - eapply trans_wl_ss_binds_etvar_a_wl in H1...
+  - eapply trans_wl_ss_binds_etvar_a_wl in H1...
+Qed.
+
 Lemma trans_wl_a_wf_typ_d_wf_typ' : forall Γ Ω θ Aᵃ Aᵈ,
   lc_typ Aᵃ ->
   nil ⊩ Γ ⇝ Ω ⫣ θ ->
@@ -1827,6 +1850,7 @@ Proof with eauto.
     dependent destruction H1...
   - dependent destruction H0...
     dependent destruction H1...
+  - dependent destruction H0... 
 Qed.
 
 Lemma trans_wl_ss_wf_typ_d_wf_typ : forall Γ Ω θ Aᵈ,
@@ -1893,8 +1917,11 @@ Proof with eauto.
     eapply trans_wl_ss_binds_etvar_a_wl...
     dependent destruction H1...
   - dependent destruction H0...
-    apply a_wf_typ__etvar...  eapply trans_wl_ss_binds_etvar_a_wl...
+    apply a_wf_typ__etvar...
+    eapply trans_wl_ss_binds_etvar_a_wl...    
     dependent destruction H1...
+  - dependent destruction H0...
+    eapply trans_wl_ss_binds_etvar_a_wl in H1...
 Qed.
 
 Lemma trans_wl_d_wf_typ_a_wf_typ : forall Γ Ω θ Aᵃ Aᵈ,
@@ -2044,17 +2071,19 @@ Proof with auto.
     eapply H0; eauto. simpl.
     rewrite_env (nil ++ (x, abind_var_typ typ_unit) :: ⌊ Γ ⌋ᵃ). 
     eapply a_wf_exp_var_binds_another with (A1:=T); eauto.
-  - dependent destruction Hwfe. constructor; eauto.
+  - dependent destruction Hwfe; constructor; eauto.
   - dependent destruction Hwfe. inst_cofinites_for d_wf_exp__tabs;
     intros; inst_cofinites_with X...
     + eapply trans_typ_dtvar_atyp_s_in_dtyp with (b:=dbind_tvar_empty); eauto.
     + rewrite_env (⌊ X ~ᵈ □ ;ᵈ Ω ⌋ᵈ). 
       eapply H0 with (Γ:=X ~ᵃ □ ;ᵃ Γ); eauto.
       constructor; eauto. econstructor...
-  - dependent destruction Hwfe. constructor; eauto.
+  - dependent destruction Hwfe; constructor; eauto.
     eapply trans_wl_a_wf_typ_d_wf_typ; eauto.
-  - dependent destruction Hwfe. constructor; eauto.
+  - dependent destruction Hwfe; constructor; eauto.
     eapply trans_wl_a_wf_typ_d_wf_typ; eauto.
+  - dependent destruction Hwfe; constructor; eauto.
+  - dependent destruction Hwfe; constructor; eauto.
 Qed.
 
 Lemma trans_wl_a_wf_exp_d_wf_exp : forall Γ Ω θ eᵃ eᵈ,
@@ -2230,14 +2259,14 @@ Proof with eauto using wf_ss_strengthen_etvar, trans_typ_strengthen_etvar.
   - inst_cofinites_for trans_exp__abs. intros.
     inst_cofinites_with x...
     eapply H0... rewrite ftvar_in_exp_open_exp_wrt_exp_upper...
-  - inst_cofinites_for trans_exp__tabs; subst; intros; inst_cofinites_with X0.
-    + rewrite_env (((X0, □) :: θ2) ++ θ1).
-      eapply H0 with (X:=X) (T:=T); eauto.
-      rewrite ftvar_in_exp_open_exp_wrt_typ_upper...
-    + rewrite_env (((X0, □) :: θ2) ++ θ1).
-      eapply trans_typ_strengthen_dtvar; eauto.
-      rewrite ftvar_in_typ_open_typ_wrt_typ_upper...
-      apply trans_typ_wf_ss in H1...
+  - inst_cofinites_for trans_exp__tabs; intros; inst_cofinites_with X0.
+    intros. rewrite_env (((X0, □) :: θ2) ++ θ1).
+    eapply H0 with (T:=T) (X:=X); eauto.
+    rewrite ftvar_in_exp_open_exp_wrt_typ_upper...
+    rewrite_env (((X0, □) :: θ2) ++ θ1).
+    eapply trans_typ_strengthen_dtvar; eauto.
+    rewrite ftvar_in_typ_open_typ_wrt_typ_upper...
+    apply trans_typ_wf_ss in H1...
 Qed.
 
 Lemma trans_conts_strengthen_etvar : forall θ1 θ2 X T csᵃ csᵈ,
@@ -2333,11 +2362,11 @@ Proof with auto using trans_typ_weaken.
   - intros. inst_cofinites_for trans_exp__abs. intros. inst_cofinites_with x.
     eapply H0...
   - intros. inst_cofinites_for trans_exp__tabs; intros; inst_cofinites_with X.
-    + rewrite_env (((X, □) :: θ3) ++ θ2 ++ θ1).
-      eapply H0... econstructor...
-    + rewrite_env (((X, □) :: θ3) ++ θ2 ++ θ1).
-      eapply trans_typ_weaken... econstructor...
-Qed. 
+    rewrite_env (((X, □) :: θ3) ++ θ2 ++ θ1).
+    eapply H0... constructor...
+    rewrite_env (((X, □) :: θ3) ++ θ2 ++ θ1).
+    eapply trans_typ_weaken... constructor...
+Qed.
 
 Lemma trans_exp_weaken_cons : forall θ X b eᵃ eᵈ,
   θ ᵉ⊩ eᵃ ⇝ eᵈ ->
@@ -2432,16 +2461,6 @@ Proof with eauto.
     rewrite_env (θ'' ++ θ2 ++ θ1). auto.
 Qed.
 
-(* Lemma trans_wl_weaken_etvar_cons : forall Γ Ω X T θ θ',
-  X ∉ ftvar_in_aworklist' Γ `union` dom θ->
-  θ ⊩ Γ ⇝ Ω ⫣ (θ' ++ θ) ->
-  d_mono_typ (ss_to_denv θ) T ->
-  (X, dbind_typ T) :: θ ⊩ Γ ⇝ Ω ⫣ (θ' ++ (X, dbind_typ T) :: θ).
-Proof.
-  intros. rewrite_env (nil ++ (X, dbind_typ T) :: θ).
-  eapply trans_wl_weaken_etvar; eauto.
-Qed. *)
-
 Lemma ftvar_in_trans_dtyp_upper : forall θ Aᵃ Aᵈ,
   θ ᵗ⊩ Aᵃ ⇝ Aᵈ ->
   ftvar_in_typ Aᵈ [<=] dom θ.
@@ -2472,8 +2491,9 @@ Proof.
     constructor. 
     apply binds_tvar_ss_binds_ss_to_denv; eauto.
   - simpl in *. constructor; eauto.
-  - simpl in *. constructor; eauto.
-  - simpl in *. constructor; eauto.
+  - simpl in *. constructor; eauto. 
+  - simpl in *. constructor; eauto. 
+  - simpl in *. constructor; eauto. 
 Qed.
 
 Lemma trans_typ_reorder_ss : forall θ θ' Aᵃ Aᵈ,
@@ -2513,6 +2533,7 @@ Proof with eauto.
     simpl in H1. econstructor...
   - dependent destruction H2...
     simpl in H1. econstructor...
+  - dependent destruction H2...
 Qed.
 
 Lemma trans_exp_reorder_ss' : forall θ θ' eᵃ eᵈ,
@@ -2535,7 +2556,8 @@ Proof with eauto.
   - simpl in *. dependent destruction H2...
     constructor...
   - dependent destruction H4.
-    inst_cofinites_for trans_exp__tabs; intros; inst_cofinites_with X.
+    inst_cofinites_for trans_exp__tabs; intros; 
+    inst_cofinites_with X.
     + assert ((X, □) :: θ ᵉ⊩ exp_anno eᵃ Aᵃ ᵉ^^ₜ ` X ⇝ exp_anno eᵈ Aᵈ ᵉ^^ₜ ` X).
       constructor; auto.
       eapply H0 with (θ':=(X, □) :: θ') in H7 ; eauto. dependent destruction H7; eauto.
@@ -2558,6 +2580,8 @@ Proof with eauto.
     constructor... eapply trans_typ_reorder_ss with (θ:=θ)...
   - simpl in *. dependent destruction H3...
     constructor... eapply trans_typ_reorder_ss with (θ:=θ)...
+  - simpl in *. dependent destruction H2...
+    constructor...
 Qed.
 
 Lemma trans_exp_reorder_ss : forall θ θ' eᵃ eᵈ,
