proof/uni_counter/algo_worklist/prop_decidability.v
@@ -2137,7 +2137,7 @@ Proof.
             destruct Hbin as [Γ1 [Γ2 Hbin]]. subst.
             assert (Hsubst: aworklist_subst (work_sub ` X (typ_arrow A1 A2) ⫤ᵃ X2 ~ᵃ ⬒ ;ᵃ X1 ~ᵃ ⬒ ;ᵃ Γ2 ⧺ X ~ᵃ ⬒ ;ᵃ Γ1) X
                                             (typ_arrow ` X1 ` X2) (X1 ~ᵃ ⬒ ;ᵃ X2 ~ᵃ ⬒ ;ᵃ Γ1) (work_sub ` X (typ_arrow A1 A2) ⫤ᵃ Γ2)).
-            { eapply a_ws1__work_stay. eapply worklist_subst_fresh_etvar_total with (Γ1 := Γ1) (Γ2 := Γ2); eauto. }
+            { eapply a_ws__work_stay. eapply worklist_subst_fresh_etvar_total with (Γ1 := Γ1) (Γ2 := Γ2); eauto. }
             assert (JgArr1: (work_sub ` X2 (subst_typ_in_typ (typ_arrow ` X1 ` X2) X A2) ⫤ᵃ work_sub (subst_typ_in_typ (typ_arrow ` X1 ` X2) X A1) ` X1 ⫤ᵃ subst_typ_in_aworklist (typ_arrow ` X1 ` X2) X Γ2 ⧺ X1 ~ᵃ ⬒ ;ᵃ X2 ~ᵃ ⬒ ;ᵃ Γ1) ⟶ᵃʷ⁎⋅ \/
                           ~ (work_sub ` X2 (subst_typ_in_typ (typ_arrow ` X1 ` X2) X A2) ⫤ᵃ work_sub (subst_typ_in_typ (typ_arrow ` X1 ` X2) X A1) ` X1 ⫤ᵃ subst_typ_in_aworklist (typ_arrow ` X1 ` X2) X Γ2 ⧺ X1 ~ᵃ ⬒ ;ᵃ X2 ~ᵃ ⬒ ;ᵃ Γ1) ⟶ᵃʷ⁎⋅).
             { eapply IHms; simpl in *; eauto.
