proof/uni_monoiu/def_extra.v
@@ -25,7 +25,7 @@ Fixpoint fvar_in_aworklist' (Γ_5:aworklist) : vars :=
     | (aworklist_cons_work Γ w) => (fvar_in_aworklist' Γ) \u (fvar_in_work w)
   end.
   
-Inductive apply_conts : conts -> typ -> work -> Prop :=
+  Inductive apply_conts : conts -> typ -> work -> Prop :=
   | apply_conts__infabs: forall A cs,
       apply_conts (conts_infabs cs) A (work_infabs A cs)
   | apply_conts__inftapp : forall A B cs,
@@ -34,13 +34,19 @@ Inductive apply_conts : conts -> typ -> work -> Prop :=
       apply_conts (conts_inftappunion A2 B cs) C1 (work_inftappunion C1 A2 B cs)
   | apply_conts__unioninftapp : forall A1 A2 cs,
       apply_conts (conts_unioninftapp A1 cs) A2 (work_unioninftapp A1 A2 cs)
+  | apply_conts__infrcdconsintersection : forall l1 A1 e2 cs,
+      apply_conts (conts_infrcdconsintersection l1 e2 cs) A1 (work_infrcdconsintersection l1 A1 e2 cs)
+  | apply_conts__intersectioninfrcdcons : forall A1 A2 cs,
+      apply_conts (conts_intersectioninfrcdcons A1 cs) A2 (work_intersectioninfrcdcons A1 A2 cs)
   | apply_conts__sub : forall A B,
       apply_conts (conts_sub B) A (work_sub A B).
 
 Inductive apply_contd : contd -> typ -> typ -> work -> Prop :=
-  | apply_contd__infapp : forall A B e c,
-      apply_contd (contd_infapp e c) A B (work_infapp A B e c)
-  | apply_contd__infabsunion : forall A2 B1 C1 c, 
-      apply_contd (contd_infabsunion A2 c) B1 C1 (work_infabsunion B1 C1 A2 c)
-  | apply_contd__unioninfabs : forall B1 B2 C1 C2 c,
-      apply_contd (contd_unioninfabs B1 C1 c) B2 C2 (work_unioninfabs B1 C1 B2 C2 c).
+  | apply_contd__infapp : forall A B e cs,
+      apply_contd (contd_infapp e cs) A B (work_infapp A B e cs)
+  | apply_contd__infabsunion : forall A2 B1 C1 cd, 
+      apply_contd (contd_infabsunion A2 cd) B1 C1 (work_infabsunion B1 C1 A2 cd)
+  | apply_contd__unioninfabs : forall B1 B2 C1 C2 cd,
+      apply_contd (contd_unioninfabs B1 C1 cd) B2 C2 (work_unioninfabs B1 C1 B2 C2 cd)
+  | apply_conted__infproj : forall A B C cs,
+      apply_contd (contd_infproj C cs) A B (work_infproj A B C cs).
